Map.v
@@ -161,8 +161,8 @@ Module Type S.
   Hint Rewrite merge_empty1 merge_empty2 using solve [ eauto 1 ].
   Hint Rewrite merge_empty1_alt merge_empty2_alt using congruence.
 
-  Hint Rewrite merge_add1 using solve [ eauto | unfold Sets.In; autorewrite with core in *; simpl in *; intuition congruence ].
-  Hint Rewrite merge_add1_alt using solve [ congruence | unfold Sets.In; autorewrite with core in *; simpl in *; intuition congruence ].
+  Hint Rewrite merge_add1 using solve [ eauto | unfold Sets.In; autorewrite with core in *; simpl in *; try (normalize_set; simpl); intuition congruence ].
+  Hint Rewrite merge_add1_alt using solve [ congruence | unfold Sets.In; autorewrite with core in *; simpl in *; try (normalize_set; simpl); intuition congruence ].
 
   Axiom includes_intro : forall K V (m1 m2 : fmap K V),
       (forall k v, m1 $? k = Some v -> m2 $? k = Some v)
